src/high/monpred_simpl.v
@@ -1,0 +1,14 @@
+From iris Require Import bi.monpred.
+
+From self.high Require Import dprop.
+
+Hint Rewrite (@monPred_at_forall thread_view_bi_index) : monpred_simpl.
+Hint Rewrite (@monPred_at_exist thread_view_bi_index) : monpred_simpl.
+Hint Rewrite (@monPred_at_and thread_view_bi_index) : monpred_simpl.
+Hint Rewrite (@monPred_at_or thread_view_bi_index) : monpred_simpl.
+Hint Rewrite (@monPred_at_wand thread_view_bi_index) : monpred_simpl.
+Hint Rewrite (@monPred_at_later thread_view_bi_index) : monpred_simpl.
+Hint Rewrite (@monPred_at_sep thread_view_bi_index) : monpred_simpl.
+Hint Rewrite (@monPred_at_objectively thread_view_bi_index) : monpred_simpl.
+Hint Rewrite (@monPred_at_pure thread_view_bi_index) : monpred_simpl.
+Ltac monPred_simpl := autorewrite with monpred_simpl.
